prove ndpa state is finite

NpTetris/Proofs/S3_2_TwoColumn/SolutionNDPA.lean
@@ -1,3 +1,5 @@
+import Mathlib.Data.Fin.Fin2
+
 import NpTetris.Proofs.S3_2_TwoColumn.NDPA
 import NpTetris.Mino
 
@@ -19,8 +21,11 @@ can be eliminated with a line clear.
 inductive FilledColumn where
 | Left
 | Right
+deriving DecidableEq
 
-instance : Fintype FilledColumn := sorry
+instance : Fintype FilledColumn where
+elems := { FilledColumn.Left, FilledColumn.Right }
+complete p := by cases p <;> simp
 
 inductive State (rows k : ℕ+) where
 /--
@@ -45,11 +50,177 @@ piece. Here are the parts of this state:
 | resolving (filled : Fin rows) (residue : List (Option FilledColumn)) (rlen: residue.length ≤ k)
 /--
 In this state, the board is ready to receive the next piece in the queue. The number of rows is
-recorded so that the machine knows whether to transition to the terminal state.
+recorded so that the machine can decide to terminate.
 -/
 | ready (filled : Fin rows)
+deriving DecidableEq
 
-instance {rows k} : Fintype (State rows k) := sorry
+def List.rec_univ {α} [Fintype α] [DecidableEq α] (k: ℕ) : Finset (List α) := by
+  induction k
+  case zero => exact {[]}
+  case succ k s =>
+    refine s ∪ ?new
+    apply Finset.map
+    case s => exact (@Finset.univ α _).product s
+    constructor
+    case toFun =>
+      intro ⟨a,xs⟩
+      refine a :: xs
+    intro p q
+    dsimp only
+    rw [List.cons.injEq]
+    rintro ⟨a,b⟩
+    ext
+    assumption
+    rw [b]
+
+theorem List.rec_univ_finite {α k} [Fintype α] [DecidableEq α]:
+  ∀ x : List α, x ∈ List.rec_univ k → x.length ≤ k
+:= by
+  unfold rec_univ
+  unfold Nat.recAux
+  dsimp
+  induction k
+  · intro x k
+    apply Nat.le_of_eq
+    apply List.length_eq_zero.mpr
+    apply Finset.eq_of_mem_singleton
+    assumption
+  case _ n ind =>
+
+  intro ls k
+  simp only [Nat.rec] at k
+  cases Finset.mem_union.mp k
+  case inr k =>
+    have ⟨_, ⟨ls_length, ls_a_x⟩⟩ := Finset.mem_map.mp k
+    have ⟨ls_length, _⟩ := Finset.mem_product.mp ls_length
+    rw [<- ls_a_x]
+    apply Nat.add_le_add_right
+    apply ind
+    assumption
+  case inl k =>
+    have := ind ls k
+    exact Nat.le_add_right_of_le (ind ls k)
+
+theorem List.rec_univ_finite' {α k} [Fintype α] [DecidableEq α]:
+  ∀ x : List α, x.length ≤ k → x ∈ List.rec_univ k
+:= by
+  unfold rec_univ
+  unfold Nat.recAux
+  dsimp only
+  induction k; simp
+  case _ n ind =>
+  intro ls ls_len
+  dsimp only [Nat.rec]
+  apply Finset.mem_union.mpr
+  cases Nat.decLt ls.length (n + 1)
+  case isFalse h =>
+    right
+    push_neg at h
+    have : 1 ≤ ls.length := by exact Nat.one_le_of_lt h
+    have : ls ≠ [] := by exact List.ne_nil_of_length_pos this
+    rw [Finset.mem_map, Prod.exists]
+    let head := ls.head this
+    exists head
+    exists ls.tail
+    constructor
+    · apply Finset.mem_product.mpr
+      simp only [Finset.mem_univ, true_and]
+      apply ind
+      apply @Nat.le_of_add_le_add_right _ 1
+      rw [List.length_tail, Nat.sub_add_cancel]
+      repeat assumption
+    · apply List.head_cons_tail
+  case isTrue h =>
+    left
+    apply ind
+    exact Nat.le_of_lt_succ h
+
+def Fin.all {n} : Finset (Fin n) := by
+  induction n
+  case zero => exact {}
+  case succ n ind =>
+    refine Finset.cons n ?set ?prf
+    · apply ind.map
+      constructor
+      case toFun => exact Fin.castSucc
+      intro p q pq
+      exact Fin.castSucc_inj.mp pq
+    · dsimp only
+      intro neg
+      have ⟨a, ⟨contra1, contra2⟩⟩ := Finset.mem_map.mp neg
+      simp at contra2
+      apply Fin.exists_castSucc_eq.mp
+      exists a
+      assumption
+
+instance Fin.instFintypeNoChoice {n} : Fintype (Fin n) where
+elems := Fin.all
+complete := by
+  unfold Fin.all
+  unfold Nat.recAux
+  induction n; simp
+  case _ a ind =>
+  dsimp at ind
+  dsimp
+  intro x
+  apply Finset.mem_cons.mpr
+  cases (Nat.decLt x.val a)
+  case isFalse h =>
+    push_neg at h
+    left
+    rw [<- Fin.cast_val_eq_self x]
+    congr
+    symm
+    apply Nat.le_antisymm h
+    apply Fin.is_le
+  case isTrue h =>
+    right
+    apply Finset.mem_map.mpr
+    exists ⟨x.val, h⟩
+    constructor
+    apply ind
+    simp only [Function.Embedding.coeFn_mk, Fin.castSucc_mk, Fin.eta]
+
+instance instFinState {rows k} : Fintype (State rows k) where
+elems := by
+  refine ?resolving ∪ ?ready
+  · have row_count : Finset (Fin rows) := Finset.univ
+    let residue : Finset (List (Option FilledColumn)) := List.rec_univ k
+    apply Finset.map
+    case s => exact row_count.product residue.attach
+    constructor
+    case toFun =>
+      intro ⟨f, ⟨g, g_residue⟩⟩
+      exact State.resolving f g (List.rec_univ_finite g g_residue)
+    intro p q
+    dsimp
+    intro pq
+    injection pq with _ k
+    ext
+    · congr
+    · rw [k]
+  · apply Finset.map
+    constructor
+    case toFun => intro rows; exact State.ready rows
+    intros _ ; simp
+    exact Finset.univ
+complete x := by
+  simp only [Finset.mem_union, Finset.mem_map, Function.Embedding.coeFn_mk, Prod.exists,
+    Subtype.exists, Finset.mem_univ, true_and]
+  cases x
+  case resolving filled residue rlen =>
+    left
+    exists filled
+    exists residue
+    exists List.rec_univ_finite' residue rlen
+    constructor
+    · apply Finset.mem_product.mpr
+      simp only [Finset.mem_univ, Finset.mem_attach, and_self]
+    · dsimp only
+  case ready filled =>
+    right
+    exists filled
 
 /-- Explanation of the types given to the NDPA:
 
@@ -68,5 +239,3 @@ step state row shape := match (state, row, shape) with
   sorry
 | (State.resolving filled residue rlen, _, none) => sorry
 | (_, _, _) => {} -- no available transitions
-
-#print axioms machine
